src/lowparse/LowParse.Steel.ArrayPtr.fst
@@ -1,0 +1,632 @@
+module LowParse.Steel.ArrayPtr
+
+module P = Steel.Pointer
+module SR = Steel.Reference
+
+let array_prop (#a: Type) (ptr: P.t a) (x: A.array a) : Tot prop =
+  A.g_get_pointer x == ptr
+
+let array (#a: Type) (ptr: P.t a) : Tot Type = (x: A.array a { array_prop ptr x })
+
+let t_array_t
+  (#a: Type)
+  (t_ptr: P.t a)
+: Tot Type0
+= if P.g_is_null t_ptr then unit else SR.ghost_ref (array t_ptr)
+
+let t_perm_t
+  (#a: Type)
+  (t_ptr: P.t a)
+: Tot Type0
+= if P.g_is_null t_ptr then unit else SR.ghost_ref perm
+
+[@@erasable]
+noeq
+type tg (#a: Type) (t_ptr: P.t a) = {
+  t_array: t_array_t t_ptr;
+  t_perm: t_perm_t t_ptr;
+}
+
+noeq
+type t a = {
+  t_ptr: P.t a;
+  t_g: tg t_ptr;
+  t_prf: squash (P.g_is_null t_ptr == false ==> P.size_v (P.base_array_len (P.base t_ptr)) < 4294967296); // TODO: remove and switch to size_t
+}
+
+let null a = {
+  t_ptr = P.null a;
+  t_g = { t_array = (); t_perm = (); };
+  t_prf = ();
+}
+
+let g_is_null x = P.g_is_null x.t_ptr
+
+let varrayptr0_refine
+  (#a: Type)
+  (x: t a)
+  (_: t_of emp)
+: Tot prop
+= g_is_null x == false
+
+let varrayptr0_payload2
+  (#a: Type)
+  (x: t a)
+  (_: t_of (emp `vrefine` varrayptr0_refine x))
+  (arp: t_of (SR.ghost_vptr #(array x.t_ptr) x.t_g.t_array `star` SR.ghost_vptr #perm x.t_g.t_perm))
+: Tot vprop
+= let (ar, p) = arp in
+  A.varrayp #a ar p
+
+[@@__steel_reduce__] // to automatically reduce t_of, necessary for the call to normal below
+let varrayptr0_payload1
+  (#a: Type)
+  (x: t a)
+  (y: t_of (emp `vrefine` varrayptr0_refine x))
+: Tot vprop
+= (SR.ghost_vptr #(array x.t_ptr) x.t_g.t_array `star` SR.ghost_vptr #perm x.t_g.t_perm) `vdep` varrayptr0_payload2 x y
+
+let varrayptr0_rewrite
+  (#a: Type)
+  (x: t a)
+  (y: normal (t_of (emp `vrefine` varrayptr0_refine x `vdep` varrayptr0_payload1 x)))
+: GTot (v a)
+= let (| _, (| (ar, p), w |) |) = y in
+  A.length_get_pointer ar;
+  {
+    array = ar;
+    contents = w;
+    perm = p;
+    prf = ();
+  }
+
+let varrayptr0
+  (#a: Type)
+  (x: t a)
+: Tot vprop
+= emp `vrefine` varrayptr0_refine x `vdep` varrayptr0_payload1 x `vrewrite` varrayptr0_rewrite x
+
+let is_arrayptr r = hp_of (varrayptr0 r)
+
+let arrayptr_sel r = sel_of (varrayptr0 r)
+
+assume
+val intro_varrayptr
+  (#opened: _)
+  (#a: Type)
+  (x: t a)
+  (ga: SR.ghost_ref (array x.t_ptr))
+  (gp: SR.ghost_ref perm)
+  (a: array x.t_ptr)
+  (p: perm)
+: SteelGhost unit opened
+    (SR.ghost_vptr ga `star` SR.ghost_vptr gp `star` A.varrayp a p)
+    (fun _ -> varrayptr x)
+    (fun h ->
+      P.g_is_null x.t_ptr == false /\
+      x.t_g.t_array == ga /\
+      x.t_g.t_perm == gp /\
+      can_be_split (SR.ghost_vptr ga `star` SR.ghost_vptr gp `star` A.varrayp a p) (SR.ghost_vptr ga) /\
+      can_be_split (SR.ghost_vptr ga `star` SR.ghost_vptr gp `star` A.varrayp a p) (SR.ghost_vptr gp) /\
+      h (SR.ghost_vptr ga) == a /\
+      h (SR.ghost_vptr gp) == p
+    )
+    (fun h _ h' ->
+      let res = h' (varrayptr x) in
+      res.array == a /\
+      res.contents == h (A.varrayp a p) /\
+      res.perm == p
+    )
+
+let intro_varrayptr'
+  (#opened: _)
+  (#b: Type)
+  (x: t b)
+  (x_ptr: P.t b)
+  (ga: SR.ghost_ref (array x_ptr))
+  (gp: SR.ghost_ref perm)
+  (a: array x_ptr)
+  (p: perm)
+: SteelGhost unit opened
+    (SR.ghost_vptr ga `star` SR.ghost_vptr gp `star` A.varrayp a p)
+    (fun _ -> varrayptr x)
+    (fun h ->
+      x_ptr == x.t_ptr /\
+      P.g_is_null x.t_ptr == false /\
+      x.t_g.t_array == ga /\
+      x.t_g.t_perm == gp /\
+      can_be_split (SR.ghost_vptr ga `star` SR.ghost_vptr gp `star` A.varrayp a p) (SR.ghost_vptr ga) /\
+      can_be_split (SR.ghost_vptr ga `star` SR.ghost_vptr gp `star` A.varrayp a p) (SR.ghost_vptr gp) /\
+      h (SR.ghost_vptr ga) == a /\
+      h (SR.ghost_vptr gp) == p
+    )
+    (fun h _ h' ->
+      let res = h' (varrayptr x) in
+      res.array == a /\
+      res.contents == h (A.varrayp a p) /\
+      res.perm == p
+    )
+=
+  let ga' : SR.ghost_ref (array x.t_ptr) = ga in
+  change_equal_slprop
+    (SR.ghost_vptr ga)
+    (SR.ghost_vptr ga');
+  intro_varrayptr x ga' gp a p
+
+[@@erasable]
+noeq
+type elim_varrayptr_t
+  (#a: Type)
+  (ptr: P.t a)
+= {
+  e_g_array: SR.ghost_ref (array ptr);
+  e_g_perm: SR.ghost_ref perm;
+  e_array: array ptr;
+  e_perm: perm;
+}
+
+assume
+val elim_varrayptr
+  (#opened: _)
+  (#a: Type)
+  (x: t a)
+: SteelGhost (elim_varrayptr_t x.t_ptr) opened
+    (varrayptr x)
+    (fun res -> SR.ghost_vptr res.e_g_array `star` SR.ghost_vptr res.e_g_perm `star` A.varrayp res.e_array res.e_perm)
+    (fun _ -> True)
+    (fun h res h' ->
+      let s = h (varrayptr x) in
+      P.g_is_null x.t_ptr == false /\
+      x.t_g.t_array == res.e_g_array /\
+      x.t_g.t_perm == res.e_g_perm /\
+      can_be_split (SR.ghost_vptr res.e_g_array `star` SR.ghost_vptr res.e_g_perm `star` A.varrayp res.e_array res.e_perm) (SR.ghost_vptr res.e_g_array) /\
+      can_be_split (SR.ghost_vptr res.e_g_array `star` SR.ghost_vptr res.e_g_perm `star` A.varrayp res.e_array res.e_perm) (SR.ghost_vptr res.e_g_perm) /\
+      h' (SR.ghost_vptr res.e_g_array) == res.e_array /\
+      h' (SR.ghost_vptr res.e_g_perm) == res.e_perm /\
+      s.array == res.e_array /\
+      s.perm == res.e_perm /\
+      h' (A.varrayp res.e_array res.e_perm) == s.contents
+    )
+
+let varrayptr_not_null
+  x
+= let res = elim_varrayptr x in
+  intro_varrayptr x res.e_g_array res.e_g_perm res.e_array res.e_perm
+
+[@@__steel_reduce__]
+let varrayptr_ghost_refs
+  (#a: Type)
+  (x: t a)
+: Tot vprop
+= if P.g_is_null x.t_ptr
+  then emp
+  else SR.ghost_vptr #(array x.t_ptr) x.t_g.t_array `star` SR.ghost_vptr #perm x.t_g.t_perm
+
+let varrayptr_ghost_refs_rewrite
+  (#a: Type)
+  (x: t a)
+  (r: t_of (varrayptr_ghost_refs x))
+: GTot (array x.t_ptr `P.gpair` perm)
+=
+  if P.g_is_null x.t_ptr
+  then
+    let _ = A.is_null_get_pointer (A.null a) in
+    A.null a `P.GPair` full_perm
+  else 
+    let r : (array x.t_ptr & perm) = r in
+    fst r `P.GPair` snd r
+
+[@@__steel_reduce__]
+let varrayptr_or_null_payload
+  (#a: Type)
+  (x: t a)
+  (r: (array x.t_ptr `P.gpair` perm))
+: Tot vprop
+= A.varrayp_or_null (P.GPair?.fst r) (P.GPair?.snd r)
+
+let varrayptr_or_null_rewrite
+  (#a: Type)
+  (x: t a)
+  (r: normal (t_of (varrayptr_ghost_refs x `vrewrite` varrayptr_ghost_refs_rewrite x `vdep` varrayptr_or_null_payload x)))
+: GTot (option (v a))
+= let (| P.GPair ar p, r |) = r in
+  match P.g_is_null x.t_ptr, r with
+  | false, Some r ->
+    A.length_get_pointer ar;
+    Some ({
+      array = ar;
+      contents = r;
+      perm = p;
+      prf = ();
+    })
+  | _ -> None
+
+[@@__steel_reduce__]
+let varrayptr_or_null0
+  (#a: Type)
+  (x: t a)
+: Tot vprop
+= varrayptr_ghost_refs x `vrewrite` varrayptr_ghost_refs_rewrite x `vdep` varrayptr_or_null_payload x `vrewrite` varrayptr_or_null_rewrite x
+
+let is_arrayptr_or_null r = hp_of (varrayptr_or_null0 r)
+
+let arrayptr_or_null_sel r = fun h -> sel_of (varrayptr_or_null0 r) h
+
+#set-options "--ide_id_info_off"
+
+let intro_varrayptr_or_null_none #_ #a x =
+  change_equal_slprop
+    emp
+    (varrayptr_ghost_refs x);
+  intro_vrewrite (varrayptr_ghost_refs x) (varrayptr_ghost_refs_rewrite x);
+  A.intro_varrayp_or_null_none (A.null a) full_perm;
+  intro_vdep
+    (varrayptr_ghost_refs x `vrewrite` varrayptr_ghost_refs_rewrite x)
+    (A.varrayp_or_null (A.null a) full_perm)
+    (varrayptr_or_null_payload x);
+  intro_vrewrite (varrayptr_ghost_refs x `vrewrite` varrayptr_ghost_refs_rewrite x `vdep` varrayptr_or_null_payload x) (varrayptr_or_null_rewrite x);
+  change_equal_slprop
+    (varrayptr_ghost_refs x `vrewrite` varrayptr_ghost_refs_rewrite x `vdep` varrayptr_or_null_payload x `vrewrite` varrayptr_or_null_rewrite x)
+    (varrayptr_or_null0 x);
+  change_slprop_rel
+    (varrayptr_or_null0 x)
+    (varrayptr_or_null x)
+    (fun u v -> u == v)
+    (fun h ->
+      assert_norm (hp_of (varrayptr_or_null0 x) == hp_of (varrayptr_or_null x));
+      assert_norm (sel_of (varrayptr_or_null0 x) h === sel_of (varrayptr_or_null x) h)
+    )
+
+let intro_varrayptr_or_null_some #_ #a x =
+  let r = elim_varrayptr x in
+  reveal_star (SR.ghost_vptr r.e_g_array) (SR.ghost_vptr r.e_g_perm);
+  change_equal_slprop
+    (SR.ghost_vptr r.e_g_array `star` SR.ghost_vptr r.e_g_perm)
+    (varrayptr_ghost_refs x);
+  intro_vrewrite (varrayptr_ghost_refs x) (varrayptr_ghost_refs_rewrite x);
+  A.intro_varrayp_or_null_some r.e_array r.e_perm;
+  intro_vdep
+    (varrayptr_ghost_refs x `vrewrite` varrayptr_ghost_refs_rewrite x)
+    (A.varrayp_or_null r.e_array r.e_perm)
+    (varrayptr_or_null_payload x);
+  intro_vrewrite (varrayptr_ghost_refs x `vrewrite` varrayptr_ghost_refs_rewrite x `vdep` varrayptr_or_null_payload x) (varrayptr_or_null_rewrite x);
+  change_equal_slprop
+    (varrayptr_ghost_refs x `vrewrite` varrayptr_ghost_refs_rewrite x `vdep` varrayptr_or_null_payload x `vrewrite` varrayptr_or_null_rewrite x)
+    (varrayptr_or_null0 x);
+  change_slprop_rel
+    (varrayptr_or_null0 x)
+    (varrayptr_or_null x)
+    (fun u v -> u == v)
+    (fun h ->
+      assert_norm (hp_of (varrayptr_or_null0 x) == hp_of (varrayptr_or_null x));
+      assert_norm (sel_of (varrayptr_or_null0 x) h === sel_of (varrayptr_or_null x) h)
+    )
+
+val intro_varrayptr_or_null
+  (#opened: _)
+  (#b: Type)
+  (x: P.t b)
+  (a: array x)
+  (p: perm)
+: SteelGhost (Ghost.erased (t b)) opened
+    (A.varrayp_or_null a p)
+    (fun res -> varrayptr_or_null res)
+    (fun _ -> 
+      P.g_is_null x == false ==> P.size_v (P.base_array_len (P.base x)) < 4294967296 // TODO: remove and switch to size_t
+    )
+    (fun h res h' ->
+      res.t_ptr == x /\
+      begin match P.g_is_null x, h (A.varrayp_or_null a p), h' (varrayptr_or_null res) with
+      | true, None, None -> True
+      | false, Some s, Some r ->
+        r.array == a /\
+        r.perm == p /\
+        r.contents == s
+      | _ -> False    
+      end
+    )
+
+let intro_varrayptr_or_null
+  #_ #b x a p
+=
+  A.is_null_get_pointer a;
+  if P.g_is_null x
+  then begin
+    A.assert_null a _;
+    let res : Ghost.erased (t b) = Ghost.hide (null _) in
+    intro_varrayptr_or_null_none res;
+    res
+  end else begin
+    A.assert_not_null a _;
+    let ga : SR.ghost_ref (array x) = SR.ghost_alloc a in
+    let gp : SR.ghost_ref perm = SR.ghost_alloc p in
+    let res : Ghost.erased (t b) = Ghost.hide ({
+      t_ptr = x;
+      t_g = {
+        t_array = ga;
+        t_perm = gp;
+      };
+      t_prf = ();
+    }) in
+    reveal_star_3 (SR.ghost_vptr ga) (SR.ghost_vptr gp) (A.varrayp a p);
+    intro_varrayptr' res x ga gp a p;
+    intro_varrayptr_or_null_some res;
+    res
+  end
+
+unfold
+let coerce (#a: Type) (x: a) (b: Type) : Pure b (requires (a == b)) (ensures (fun y -> a == b /\ x == y)) = x
+
+unfold
+let coerce2 (#a: Type) (x: a) (b: Type) (sq: squash (a == b)) : Tot b = x
+
+let elim_varrayptr_or_null_some #_ #a x =
+  change_slprop_rel
+    (varrayptr_or_null x)
+    (varrayptr_or_null0 x)
+    (fun u v -> u == v)
+    (fun h ->
+      assert_norm (hp_of (varrayptr_or_null0 x) == hp_of (varrayptr_or_null x));
+      assert_norm (sel_of (varrayptr_or_null0 x) h === sel_of (varrayptr_or_null x) h)
+    );
+  elim_vrewrite
+    (varrayptr_ghost_refs x `vrewrite` varrayptr_ghost_refs_rewrite x `vdep` varrayptr_or_null_payload x) (varrayptr_or_null_rewrite x);
+  let _ : squash (P.g_is_null x.t_ptr == false) = () in
+  let pa : squash (t_array_t x.t_ptr == SR.ghost_ref (array x.t_ptr)) = () in
+  let pp : squash (t_perm_t x.t_ptr == SR.ghost_ref perm) = () in
+  let ga : SR.ghost_ref (array x.t_ptr) = coerce2 x.t_g.t_array (SR.ghost_ref (array x.t_ptr)) pa in
+  let gp : SR.ghost_ref perm = coerce2 x.t_g.t_perm (SR.ghost_ref perm) pp in
+  let g : Ghost.erased (P.gpair (array x.t_ptr) perm) = elim_vdep
+    (varrayptr_ghost_refs x `vrewrite` varrayptr_ghost_refs_rewrite x)
+    (varrayptr_or_null_payload x)
+  in
+  elim_vrewrite (varrayptr_ghost_refs x) (varrayptr_ghost_refs_rewrite x);
+  change_equal_slprop
+    (varrayptr_ghost_refs x)
+    (SR.ghost_vptr ga `star` SR.ghost_vptr gp);
+  SR.ghost_vptr ga `reveal_star` SR.ghost_vptr gp;
+  A.is_null_get_pointer (P.GPair?.fst g);
+  change_equal_slprop
+    (varrayptr_or_null_payload x g)
+    (A.varrayp_or_null (P.GPair?.fst g) (P.GPair?.snd g));
+  A.assert_not_null (P.GPair?.fst g) (P.GPair?.snd g);
+  reveal_star_3 (SR.ghost_vptr ga) (SR.ghost_vptr gp) (A.varrayp (P.GPair?.fst g) (P.GPair?.snd g));
+  intro_varrayptr x ga gp (P.GPair?.fst g) (P.GPair?.snd g)
+
+let elim_varrayptr_or_null_none #_ #a x =
+  change_slprop_rel
+    (varrayptr_or_null x)
+    (varrayptr_or_null0 x)
+    (fun u v -> u == v)
+    (fun h ->
+      assert_norm (hp_of (varrayptr_or_null0 x) == hp_of (varrayptr_or_null x));
+      assert_norm (sel_of (varrayptr_or_null0 x) h === sel_of (varrayptr_or_null x) h)
+    );
+  elim_vrewrite
+    (varrayptr_ghost_refs x `vrewrite` varrayptr_ghost_refs_rewrite x `vdep` varrayptr_or_null_payload x) (varrayptr_or_null_rewrite x);
+  let g : Ghost.erased (P.gpair (array x.t_ptr) perm) = elim_vdep
+    (varrayptr_ghost_refs x `vrewrite` varrayptr_ghost_refs_rewrite x)
+    (varrayptr_or_null_payload x)
+  in
+  change_equal_slprop
+    (varrayptr_or_null_payload x g)
+    (A.varrayp_or_null (P.GPair?.fst g) (P.GPair?.snd g));
+  A.is_null_get_pointer (P.GPair?.fst g);
+  if P.g_is_null x.t_ptr
+  then begin
+    A.assert_null (P.GPair?.fst g) (P.GPair?.snd g);
+    elim_vrewrite (varrayptr_ghost_refs x) (varrayptr_ghost_refs_rewrite x);
+    change_equal_slprop
+      (varrayptr_ghost_refs x)
+      emp
+  end else begin
+    A.assert_not_null (P.GPair?.fst g) (P.GPair?.snd g);
+    assert False;
+    change_slprop_rel
+      ((varrayptr_ghost_refs x `vrewrite` varrayptr_ghost_refs_rewrite x) `star` A.varrayp (P.GPair?.fst g) (P.GPair?.snd g))
+      emp
+      (fun _ _ -> False)
+      (fun _ -> ())
+  end
+
+let is_null_none
+  (#opened: _)
+  (#a: Type)
+  (x: t a)
+: SteelGhost unit opened
+    (varrayptr_or_null x)
+    (fun _ -> varrayptr_or_null x)
+    (fun _ -> True)
+    (fun h _ h' ->
+      let s = h (varrayptr_or_null x) in
+      h' (varrayptr_or_null x) == s /\
+      g_is_null x == None? s
+    )
+=
+  if g_is_null x
+  then begin
+    elim_varrayptr_or_null_none x;
+    intro_varrayptr_or_null_none x
+  end else begin
+    elim_varrayptr_or_null_some x;
+    intro_varrayptr_or_null_some x
+  end
+
+let is_null
+  #_ #a x
+=
+  is_null_none x;
+  change_slprop_rel
+    (varrayptr_or_null x)
+    (varrayptr_or_null0 x)
+    (fun u v -> u == v)
+    (fun h ->
+      assert_norm (hp_of (varrayptr_or_null0 x) == hp_of (varrayptr_or_null x));
+      assert_norm (sel_of (varrayptr_or_null0 x) h === sel_of (varrayptr_or_null x) h)
+    );
+  elim_vrewrite
+    (varrayptr_ghost_refs x `vrewrite` varrayptr_ghost_refs_rewrite x `vdep` varrayptr_or_null_payload x) (varrayptr_or_null_rewrite x);
+  let g : Ghost.erased (P.gpair (array x.t_ptr) perm) = elim_vdep
+    (varrayptr_ghost_refs x `vrewrite` varrayptr_ghost_refs_rewrite x)
+    (varrayptr_or_null_payload x)
+  in
+  change_equal_slprop
+    (varrayptr_or_null_payload x g)
+    (A.varrayp_or_null (Ghost.reveal (Ghost.hide (P.GPair?.fst g))) (P.GPair?.snd g));
+  let ar = A.reveal x.t_ptr (Ghost.hide (P.GPair?.fst g)) (P.GPair?.snd g) in
+  A.is_null_get_pointer ar;
+  let res = A.is_null ar _ in
+  intro_vdep
+    (varrayptr_ghost_refs x `vrewrite` varrayptr_ghost_refs_rewrite x)
+    (A.varrayp_or_null ar (P.GPair?.snd g))
+    (varrayptr_or_null_payload x);
+  intro_vrewrite
+    (varrayptr_ghost_refs x `vrewrite` varrayptr_ghost_refs_rewrite x `vdep` varrayptr_or_null_payload x) (varrayptr_or_null_rewrite x);
+  change_slprop_rel
+    (varrayptr_or_null0 x)
+    (varrayptr_or_null x)
+    (fun u v -> u == v)
+    (fun h ->
+      assert_norm (hp_of (varrayptr_or_null0 x) == hp_of (varrayptr_or_null x));
+      assert_norm (sel_of (varrayptr_or_null0 x) h === sel_of (varrayptr_or_null x) h)
+    );
+  return res
+
+let join al ar =
+  let el = elim_varrayptr al in
+  let er = elim_varrayptr ar in
+  SR.ghost_free er.e_g_array;
+  SR.ghost_free er.e_g_perm;
+  change_equal_slprop
+    (A.varrayp er.e_array er.e_perm)
+    (A.varrayp er.e_array el.e_perm);
+  let a' = A.join' el.e_array er.e_array _ in
+  A.length_get_pointer a';
+  A.get_pointer_merge el.e_array er.e_array;
+  SR.ghost_write el.e_g_array (Ghost.reveal a');
+  reveal_star_3 (SR.ghost_vptr el.e_g_array) (SR.ghost_vptr el.e_g_perm) (A.varrayp a' el.e_perm);
+  intro_varrayptr al el.e_g_array el.e_g_perm a' el.e_perm
+
+let split x i =
+  varrayptr_not_null x;
+  let e = elim_varrayptr x in
+  change_equal_slprop
+    (A.varrayp e.e_array e.e_perm)
+    (A.varrayp (Ghost.hide e.e_array) e.e_perm);
+  A.intro_varrayp_or_null_some (Ghost.hide e.e_array) e.e_perm;
+  let a = A.reveal x.t_ptr (Ghost.hide e.e_array) _ in
+  A.assert_not_null a e.e_perm;
+  let j = P.mk_size_t i in
+  let alar = A.splitp a _ j in
+  A.get_pointer_gsplit a j;
+  SR.ghost_write e.e_g_array (fst alar);
+  reveal_star_3 (SR.ghost_vptr e.e_g_array) (SR.ghost_vptr e.e_g_perm) (A.varrayp (fst alar) e.e_perm);
+  intro_varrayptr x e.e_g_array e.e_g_perm (fst alar) e.e_perm;
+  let ar = snd alar in
+  change_equal_slprop
+    (A.varrayp (snd alar) e.e_perm)
+    (A.varrayp ar e.e_perm);
+  A.intro_varrayp_or_null_some ar _;
+  let pr = A.get_pointer ar _ in
+  A.assert_not_null ar _;
+  let ga : SR.ghost_ref (array pr) = SR.ghost_alloc ar in
+  let gp : SR.ghost_ref perm = SR.ghost_alloc e.e_perm in
+  let res = ({
+    t_ptr = pr;
+    t_g = {
+      t_array = ga;
+      t_perm = gp;
+    };
+    t_prf = ();
+  }) in
+  reveal_star_3 (SR.ghost_vptr ga) (SR.ghost_vptr gp) (A.varrayp ar e.e_perm);
+  intro_varrayptr' res pr ga gp ar e.e_perm;
+  return res
+
+let alloc x n =
+  let ar = A.malloc x (P.mk_size_t n) in
+  let p = A.get_pointer ar _ in
+  A.is_null_get_pointer ar;
+  A.length_get_pointer ar;
+  let g = intro_varrayptr_or_null p ar _ in
+  let res = {
+    t_ptr = p;
+    t_g = g.t_g;
+    t_prf = g.t_prf;
+  } in
+  change_equal_slprop
+    (varrayptr_or_null g)
+    (varrayptr_or_null res);
+  return res
+
+let index #b r i =
+  let e = elim_varrayptr r in
+  let g : Ghost.erased (A.array b) = Ghost.hide e.e_array in
+  change_equal_slprop
+    (A.varrayp e.e_array e.e_perm)
+    (A.varrayp g e.e_perm);
+  A.intro_varrayp_or_null_some g _;
+  let a = A.reveal r.t_ptr g _ in
+  A.assert_not_null a _;
+  let res = A.indexp a _ (P.mk_size_t i) in
+  intro_varrayptr r e.e_g_array e.e_g_perm a _;
+  return res
+
+let upd #b r i v =
+  let e = elim_varrayptr r in
+  let g : Ghost.erased (A.array b) = Ghost.hide e.e_array in
+  change_equal_slprop
+    (A.varrayp e.e_array e.e_perm)
+    (A.varray g);
+  A.intro_varrayp_or_null_some g _;
+  let a = A.reveal r.t_ptr g _ in
+  A.assert_not_null a _;
+  A.upd a (P.mk_size_t i) v;
+  intro_varrayptr r e.e_g_array e.e_g_perm a _
+
+let free r =
+  let e = elim_varrayptr r in
+  SR.ghost_free e.e_g_array;
+  SR.ghost_free e.e_g_perm;
+  let g : Ghost.erased (A.array _) = Ghost.hide e.e_array in
+  change_equal_slprop
+    (A.varrayp e.e_array e.e_perm)
+    (A.varray g);
+  A.intro_varrayp_or_null_some g _;
+  let a = A.reveal r.t_ptr g _ in
+  A.assert_not_null a _;
+  A.free a
+
+let share r =
+  let e = elim_varrayptr r in
+  let p = A.share e.e_array _ in
+  SR.ghost_write e.e_g_perm p;
+  reveal_star_3 (SR.ghost_vptr e.e_g_array) (SR.ghost_vptr e.e_g_perm) (A.varrayp e.e_array p);
+  intro_varrayptr r e.e_g_array e.e_g_perm e.e_array p;
+  let ga : SR.ghost_ref (array r.t_ptr) = SR.ghost_alloc e.e_array in
+  let gp : SR.ghost_ref perm = SR.ghost_alloc p in
+  let res = {
+    t_ptr = r.t_ptr;
+    t_g = {
+      t_array = ga;
+      t_perm = gp;
+    };
+    t_prf = ();
+  } in
+  reveal_star_3 (SR.ghost_vptr ga) (SR.ghost_vptr gp) (A.varrayp e.e_array p);
+  intro_varrayptr' res r.t_ptr ga gp e.e_array p;
+  return res
+
+let gather r1 r2 =
+  let e1 = elim_varrayptr r1 in
+  let e2 = elim_varrayptr r2 in
+  SR.ghost_free e2.e_g_array;
+  SR.ghost_free e2.e_g_perm;
+  assert (e2.e_array == e1.e_array);
+  change_equal_slprop
+    (A.varrayp e2.e_array e2.e_perm)
+    (A.varrayp e1.e_array e2.e_perm);
+  let p = A.gather e1.e_array e1.e_perm e2.e_perm in
+  SR.ghost_write e1.e_g_perm p;
+  reveal_star_3 (SR.ghost_vptr e1.e_g_array) (SR.ghost_vptr e1.e_g_perm) (A.varrayp e1.e_array p);
+  intro_varrayptr r1 e1.e_g_array e1.e_g_perm e1.e_array p
